share/steel/examples/pulse/parallel/SingleGhostTask.fsti
@@ -31,23 +31,24 @@ stt_atomic unit #Unobservable (singleton i)
 
 type task_status = | Todo | Ongoing | Done
 
-let thunk bpre bpost
+let thunk bpre bpost (f: perm) (status_pool: ref bool)
   = unit -> stt unit
   (GR.pts_to bpre #one_half true ** GR.pts_to bpost #one_half false)
-  (fun () -> GR.pts_to bpre #one_half false ** GR.pts_to bpost #one_half true)
+  (fun () -> GR.pts_to bpre #one_half false ** GR.pts_to bpost #one_half true ** pts_to status_pool #f true)
 
 let lock_task (bdone: ref bool): vprop =
   exists* v f. pts_to bdone #f v ** pure (if not v then f == one_half else true)
 
-type task =
-    (bpre: GR.ref bool & bpost: GR.ref bool & thunk bpre bpost & (bdone: ref bool & Lock.lock (lock_task bdone)) & bclaimed: GR.ref bool)
+type task status_pool =
+    (bpre: GR.ref bool & bpost: GR.ref bool & (f: perm & thunk bpre bpost f status_pool) & (bdone: ref bool & Lock.lock (lock_task bdone)) & bclaimed: GR.ref bool)
+
+
+val create_task (#pre #post: vprop) (f: (unit -> stt unit pre (fun () -> post))) (p: perm) (status_pool: ref bool):
+    stt (t: task status_pool & inv (guarded_inv t._2 post))
+    (pre ** pts_to status_pool #p true)
+    (fun r -> GR.pts_to r._1._1 #one_half true ** GR.pts_to r._1._2 #one_half false ** pts_to r._1._4._1 #one_half false ** GR.pts_to r._1._5 false)
 
 let x = ()
-
-val create_task (#pre #post: vprop) (f: (unit -> stt unit pre (fun () -> post))):
-    stt (t: task & inv (guarded_inv t._2 post))
-    pre
-    (fun r -> GR.pts_to r._1._1 #one_half true ** GR.pts_to r._1._2 #one_half false ** pts_to r._1._4._1 #one_half false ** GR.pts_to r._1._5 false)
 
 type extended_task: Type =
     task & task_status
